formalization/Typing.v
@@ -18,16 +18,18 @@ Import BasicTyping.
 Import RefinementType.
 Import Denotation.
 Import Instantiation.
-Import Substitution.
 
 (* TODO: wf_am? *)
 
 (** Well-formedness *)
+Definition wf_am (Γ: listctx pty) (A: am): Prop := closed_am (ctxdom ⦑ Γ ⦒) A.
+
 Inductive wf_pty: listctx pty -> pty -> Prop :=
 | wf_pty_base: forall Γ b ϕ,
-    closed_pty (ctxdom ⦑ Γ ⦒) {v: b | ϕ } ->  wf_pty Γ {v: b | ϕ }
+    closed_pty (ctxdom ⦑ Γ ⦒) {v: b | ϕ } -> wf_pty Γ {v: b | ϕ }
 | wf_pty_arr: forall Γ ρ T A B (L: aset),
-    (* NOTE: ρ? *)
+    wf_pty Γ ρ ->
+    wf_am Γ A ->
     amlist_typed B T ->
     (forall x, x ∉ L ->
           (forall Bi ρi, In (Bi, ρi) B ->
@@ -39,9 +41,7 @@ Inductive wf_pty: listctx pty -> pty -> Prop :=
 Inductive wf_hty: listctx pty -> hty -> Prop :=
 | wf_hty_: forall Γ T A B,
     amlist_typed B T ->
-    (forall Bi ρi, In (Bi, ρi) B ->
-              wf_pty Γ ρi
-    ) ->
+    (forall Ai ρi, In (Ai, ρi) B -> wf_am Γ Ai /\ wf_pty Γ ρi) ->
     wf_hty Γ [: T | A ⇒ B ].
 
 Notation " Γ '⊢WF' τ " := (wf_hty Γ τ) (at level 20, τ constr, Γ constr).
@@ -49,15 +49,13 @@ Notation " Γ '⊢WFp' τ " := (wf_pty Γ τ) (at level 20, τ constr, Γ constr
 
 Definition subtyping (Γ: listctx pty) (τ1 τ2: hty) : Prop :=
   (* Assume [τ1] and [τ2] are valid [hty]s. *)
-  forall env, ctxRst Γ env ->
-  (* NOTE: why not use value? *)
-         forall e, ⟦ msubst hty_subst env τ1 ⟧ (tm_msubst env e) ->
-              ⟦ msubst hty_subst env τ2 ⟧ (tm_msubst env e).
+  forall Γv, ctxRst Γ Γv -> forall v,⟦(m{ Γv }h) τ1⟧ ((m{ Γv }v) v) → ⟦(m{ Γv }h) τ2⟧ ((m{ Γv }v) v).
 
 Notation " Γ '⊢' τ1 '⪡' τ2 " := (subtyping Γ τ1 τ2) (at level 20, τ1 constr, τ2 constr, Γ constr).
 
 Reserved Notation "Γ '⊢' e '⋮t' τ" (at level 20).
 Reserved Notation "Γ '⊢' e '⋮v' τ"  (at level 20).
+
 
 Definition A_ρa_B_ρb_list_A_ρa (l: list (am * pty) ) (tril: list (am * pty * am * pty)) :=
   forall A ρa, In (A, ρa) l <-> (exists B ρb, In (A, ρa, B, ρb) tril).
@@ -136,11 +134,11 @@ Scheme value_type_check_rec := Induction for value_type_check Sort Prop
     with term_type_check_rec := Induction for term_type_check Sort Prop.
 
 Lemma value_typing_regular: forall (Γ: listctx pty) (v: value) (ρ: pty),
-    Γ ⊢ v ⋮v ρ -> ⌊ Γ ⌋* ⊢t v ⋮v ⌊ ρ ⌋.
+    Γ ⊢ v ⋮v ρ -> ⌊ Γ ⌋* ⊢t v ⋮v ⌊ ρ ⌋ /\ wf_pty Γ ρ.
 Admitted.
 
 Lemma tm_typing_regular: forall (Γ: listctx pty) (e: tm) (τ: hty),
-    Γ ⊢ e ⋮t τ -> ⌊ Γ ⌋* ⊢t e ⋮t ⌊ τ ⌋.
+    Γ ⊢ e ⋮t τ -> ⌊ Γ ⌋* ⊢t e ⋮t ⌊ τ ⌋ /\ wf_hty Γ τ.
 Admitted.
 
 Lemma well_formed_builtin_typing: forall op ρx A B ρ,
@@ -158,64 +156,90 @@ Lemma reduction_tlete:  forall e_x e α β v,
 Admitted.
 
 (* I have proved this lemma in Poirot. *)
-Lemma msubst_open: forall (env: env) e (v_x: value) (x: atom),
-    x # (dom env ∪ stale e ∪ stale v_x) ->
-    tm_msubst env e ^t^ v_x = tm_msubst (<[x := v_x]> env) (e ^t^ x).
+Lemma msubst_open: forall (Γv: env) e (v_x: value) (x: atom),
+    x # (dom Γv ∪ stale e ∪ stale v_x) ->
+    (m{Γv}t) e ^t^ v_x = (m{<[x:=v_x]> Γv}t) (e ^t^ x).
+Admitted.
+
+Lemma msubst_hty: forall (Γv: env) T A B, m{Γv}h [:T|A⇒B] = [:T|m{Γv}a A ⇒ m{Γv}pa B].
+Admitted.
+
+Lemma msubst_concat: forall (Γv: env) A1 A2, m{Γv}a (aconcat A1 A2) = (aconcat (m{Γv}a A1) (m{Γv}a A2)).
+Admitted.
+
+Lemma in_msubst: forall (Γv: env) (A: am) (ρ: pty) (B: list (am * pty)),
+    In (A, ρ) (m{Γv}pa B) <-> exists A' ρ', A = m{Γv}a A' /\ ρ = m{Γv}p ρ' /\ In (A', ρ') B.
+Admitted.
+
+Definition subst4 Γv (x: am * pty * am * pty) :=
+  match x with
+    | (A, ρa, B, ρb) => (m{Γv}a A, m{Γv}p ρa, m{Γv}a B, m{Γv}p ρb)
+  end.
+
+Lemma in_msubst4: forall (Γv: env) (A1: am) (ρ1: pty) (A2: am) (ρ2: pty) (B4: list (am * pty * am * pty)),
+    In (A1, ρ1, A2, ρ2) (List.map (subst4 Γv) B4) ->
+    exists A1' ρ1' A2' ρ2',
+      A1 = m{Γv}a A1' /\ ρ1 = m{Γv}p ρ1' /\ A2 = m{Γv}a A2' /\ ρ2 = m{Γv}p ρ2' /\ In (A1', ρ1', A2', ρ2') B4.
 Admitted.
 
 Lemma am_concat: forall A B α β,
-  (a⟦A⟧) α ->
-  (a⟦B⟧) β ->
-  (a⟦ aconcat A B ⟧) (α +;+ β).
+  (a⟦A⟧) α -> (a⟦B⟧) β -> (a⟦ aconcat A B ⟧) (α +;+ β).
 Admitted.
+
+Lemma am_denotation_fv: forall Γv x v_x A,
+    x ∉ stale A -> forall α, a⟦(m{<[x:=v_x]> Γv}a) A⟧ α <-> a⟦(m{Γv}a) A⟧ α.
+Admitted.
+
+Lemma in_singleton {T1 T2: Type}: forall (a1 a1': T1) (a2 a2': T2), In (a1, a2) [(a1', a2')] -> a1 = a1' /\ a2 = a2'.
+Proof.
+  intros. inversion H. inversion H0; subst; auto. inversion H0.
+Qed.
 
 Theorem fundamental: forall (Γ: listctx pty) (e: tm) (τ: hty),
     Γ ⊢ e ⋮t τ ->
     (* NOTE: [τ] being valid should be a regularity lemma. *)
-    forall env, ctxRst Γ env -> ⟦ msubst hty_subst env τ ⟧ (tm_msubst env e).
+    forall Γv, ctxRst Γ Γv -> ⟦ msubst hty_subst Γv τ ⟧ (msubst tm_subst Γv e).
 Proof.
   apply (term_type_check_rec
            (* NOTE: should this be the denotation of [pty]? *)
            (fun Γ (v: value) ρ _ =>
-              forall env,
-                ctxRst Γ env ->
-                ⟦ msubst hty_subst env (pty_to_rty ρ) ⟧ (value_msubst env v))
+              forall Γv, ctxRst Γ Γv -> ⟦ m{Γv}h (pty_to_rty ρ) ⟧ (m{Γv}v v))
            (fun Γ e (τ: hty) _ =>
-              forall env,
-                ctxRst Γ env -> ⟦ msubst hty_subst env τ ⟧ (tm_msubst env e))
-        ); intros.
+              forall Γv, ctxRst Γ Γv -> ⟦ m{Γv}h τ ⟧ (m{Γv}t e))
+        ).
   - admit.
   - admit.
   - admit.
   - admit.
   - admit.
   - admit.
-  - auto_pose_fv x. repeat specialize_with x.
-    (* clear t t0. *)
-    (* assert ((tm_msubst env (tlete e_x e)) = (tlete (tm_msubst env e_x) (tm_msubst env e))) as Hrewrite; auto. *)
-    (* rewrite Hrewrite. clear Hrewrite. *)
-    (* simpl. *)
-    (* intros. *)
-    (* rewrite reduction_tlete in H6. mydestr; subst. rewrite msubst_open with (x:=x) in H8. 2: { admit. } *)
-    (* specialize (H env st H1 H2). simpl in H. *)
-    (* assert (amlist_typed Bx_ρx Tx) as HH1. admit. *)
-    (* rename x0 into βx. rename x2 into v_x. rename x1 into βe. *)
-    (* specialize (H HH1 α βx v_x H5 H7). destruct H as (Bxi & ρxi & HinBx_ρx & Hβx & Hv_x). *)
-    (* apply a in HinBx_ρx. destruct HinBx_ρx as (Bi & ρi & Hin). *)
-    (* specialize (H0 _ _ _ _ Hin (<[ x := v_x]> env) st). (* Here st should be 1: st when v_x is a function 2: <[ x := v_x]> st when v_x is a constant *) *)
-    (* assert (ctxRst (Γ ++ [(x, ρxi)]) (<[x:=v_x]> env)) as HH2. admit. *)
-    (* assert (st⫕<[x:=v_x]> env) as HH3. admit. *)
-    (* specialize (H0 HH2 HH3). simpl in H0. *)
-    (* assert (amlist_typed [(Bi, ρi)] T) as HH4. admit. *)
-    (* specialize (H0 HH4 (α +;+ βx) βe v). *)
-    (* assert (closed_am 0 (dom st) (aconcat A Bxi)) as HH5. admit. *)
-    (* assert ( *)
-    (*     (closed_am 0 (dom st) (aconcat A Bxi)) /\ *)
-    (*     (∃ α1 α2 : trace, α +;+ βx = α1 +;+ α2 ∧ ({0;b∅;st}a⟦A⟧) α1 ∧ ({0;b∅;st}a⟦Bxi⟧) α2)) as Hconcat. *)
-    (* { split; eauto. } *)
-    (* specialize (H0 Hconcat H8). clear Hconcat. *)
-    (* destruct H0 as (Bi' & ρi' & Heq & Hβe & Hv). destruct Heq. 2: { inversion H. } inversion H; subst. *)
-    (* rename Bi' into Bi. rename ρi' into ρi. *)
-    (* exists (aconcat Bxi Bi), ρi. *)
-    (* split. apply a0; eauto. split; auto. apply am_concat; auto. *)
+  - intros Γ e_x e Tx A T Bx_ρx BxB_ρ Bx_ρx_B_ρ L HWFe_x _ HDe_x Hin1 Hin2 _ He Γv HΓv.
+    auto_pose_fv x. repeat specialize_with x.
+    assert (m{Γv}t (tlete e_x e) = tlete ((m{Γv}t) e_x) ((m{Γv}t) e)) as Hrewrite.
+    { admit. } rewrite Hrewrite. clear Hrewrite.
+    rewrite msubst_hty.
+    simpl. intros HBtyped α β v HDα Hstepv.
+    rewrite reduction_tlete in Hstepv. destruct Hstepv as (βx & βe & v_x & Htmp & Hstepv_x & Hstepv). subst.
+    rewrite msubst_open with (x:=x) in Hstepv. 2: { admit. }
+    specialize (HDe_x _ HΓv). rewrite msubst_hty in HDe_x.
+    assert (amlist_typed ((m{Γv}pa) Bx_ρx) Tx) as HH1. admit.
+    specialize (HDe_x HH1 _ _ _ HDα Hstepv_x).
+    destruct HDe_x as (Bxi' & ρxi' & HinBx_ρx & Hβx & Hv_x).
+    apply in_msubst in HinBx_ρx. destruct HinBx_ρx as (Bxi & ρxi & Htmp0 & Htmp1 & HinBx_ρx); subst.
+    apply Hin1 in HinBx_ρx. destruct HinBx_ρx as (Bi & ρi & Hin). clear Hin1.
+    assert (ctxRst (Γ ++ [(x, ρxi)]) (<[x:=v_x]> Γv)) as HH2. constructor; auto. admit.
+    specialize (He _ _ _ _ Hin (<[ x := v_x]> Γv) HH2). rewrite msubst_hty in He.
+    assert (amlist_typed ((m{<[x:=v_x]> Γv}pa) [(Bi, ρi)]) T) as HH3. admit.
+    specialize (He HH3 (α +;+ βx) βe v).
+    assert (x ∉ stale Bxi). admit.
+    assert ((a⟦(m{<[x:=v_x]> Γv}a) (aconcat A Bxi)⟧) (α +;+ βx)) as Hconcat.
+    { rewrite am_denotation_fv; try fast_set_solver. rewrite msubst_concat.
+      apply am_concat; auto. }
+    specialize (He Hconcat Hstepv). destruct He as (Bi'' & ρi'' & Hini & Hβe & Hv).
+    apply in_msubst in Hini. destruct Hini as (Bi' & ρi' & Htmp0 & Htmp1 & Hini); subst.
+    apply in_singleton in Hini. mydestr; subst.
+    assert (In ((aconcat Bxi Bi), ρi) BxB_ρ) as Hinii. { apply Hin2. eauto. }
+    exists (m{<[x:=v_x]> Γv}a (aconcat Bxi Bi)), (m{<[x:=v_x]> Γv}p ρi).
+    split. rewrite in_msubst. exists (aconcat Bxi Bi), ρxi. admit.
+    split; auto. rewrite msubst_concat. apply am_concat; auto. rewrite am_denotation_fv; auto.
 Admitted.
