formalization/Instantiation.v
@@ -16,29 +16,32 @@ Import Equation.
 
 Definition env := amap value.
 
-Fixpoint value_msubst (env: env) (v : value): value :=
-  match v with
-  | vconst _ => v
-  | vfvar y => match env !! y with
-              | None => v
-              | Some s => s
-              end
-  | vbvar _ => v
-  | vlam T e => vlam T (tm_msubst env e)
-  | vfix Tf e => vfix Tf (tm_msubst env e)
-  end
-with tm_msubst (env: env) (e : tm): tm :=
-       match e with
-       | treturn v => treturn (value_msubst env v)
-       | tlete e1 e2 => tlete (tm_msubst env e1) (tm_msubst env e2)
-       | tletapp v1 v2 e => tletapp (value_msubst env v1) (value_msubst env v2) (tm_msubst env e)
-       | tleteffop op v1 e => tleteffop op (value_msubst env v1) (tm_msubst env e)
-       | tmatchb v e1 e2 => tmatchb (value_msubst env v) (tm_msubst env e1) (tm_msubst env e2)
-       end.
+(* Fixpoint value_msubst (env: env) (v : value): value := *)
+(*   match v with *)
+(*   | vconst _ => v *)
+(*   | vfvar y => match env !! y with *)
+(*               | None => v *)
+(*               | Some s => s *)
+(*               end *)
+(*   | vbvar _ => v *)
+(*   | vlam T e => vlam T (tm_msubst env e) *)
+(*   | vfix Tf e => vfix Tf (tm_msubst env e) *)
+(*   end *)
+(* with tm_msubst (env: env) (e : tm): tm := *)
+(*        match e with *)
+(*        | treturn v => treturn (value_msubst env v) *)
+(*        | tlete e1 e2 => tlete (tm_msubst env e1) (tm_msubst env e2) *)
+(*        | tletapp v1 v2 e => tletapp (value_msubst env v1) (value_msubst env v2) (tm_msubst env e) *)
+(*        | tleteffop op v1 e => tleteffop op (value_msubst env v1) (tm_msubst env e) *)
+(*        | tmatchb v e1 e2 => tmatchb (value_msubst env v) (tm_msubst env e1) (tm_msubst env e2) *)
+(*        end. *)
 
 Definition msubst {A} (subst : atom -> value -> A -> A)
                   (env : env) (a : A) : A :=
   map_fold subst a env.
+
+(* Definition value_msubst := msubst value_subst. *)
+(* Definition tm_msubst := msubst tm_subst. *)
 
 Definition instantiation (Γ: amap ty) (Γv: env) :=
   forall (x: atom),
@@ -53,8 +56,8 @@ Definition instantiation (Γ: amap ty) (Γv: env) :=
 
 Definition termRraw (α: trace) Γ e e' :=
   forall Γv β (v: value), instantiation Γ Γv ->
-                   α ⊧ tm_msubst Γv e ↪*{ β } v ->
-                   α ⊧ tm_msubst Γv e' ↪*{ β } v.
+                   α ⊧ msubst tm_subst Γv e ↪*{ β } v ->
+                   α ⊧ msubst tm_subst Γv e' ↪*{ β } v.
 
 Inductive termR: trace -> amap ty -> ty -> tm -> tm -> Prop :=
 | termR_c: forall α Γ T (e e': tm),
